Zero $2$nd derivative at ends. 
$$S_{1}''(X_{1}) = 0$$
$$S_{n-1}''(X_{n}) = 0
$$
Earlier, we had the 2nd derivative, so use it to get..
$$S_{1}''(X_{1})= 2c_{1} + 6d_{1}(x_{1}- x_{i}) = 0$$
So, 
$$c_{1}= \frac{3y_{i}' - 2s - s_{2}}{\Delta x_{i}}= 0
$$
Simplifying this gives us:
$$s_{1}+ \frac{1}{2}s_{2}= \frac{3}{2}y_{i}'$$
Likewise for $S_{n-1}''(X_{n)}= 0$, 

$$S_{n-1}''(X_{n})= 2c_{n-1} + 6d_{n-1}(x_{n}- x_{n-1}) = 0$$
Expand $c$ and $d$: 
$$$$$$2\left(\frac{3y_{n-1}' - 2s_{n-1}- s_n}{\Delta x_{n-1}}\right)+ 6\left(\frac{s_{n}+s_{n-1}- 2y_{n-1}'}{\Delta x_{i+1}}\right) = 0$$
